Add a built-in function for "select" (strict conditional)
The built-in is called `EF_select` and has type `(int, T, T) -> T` for
a given Cminor type T.

During instruction selection, it is turned into an `Osel` operation if
available, otherwise into an if/then/else.

arm/AsmToJSON.ml
@@ -179,7 +179,8 @@ let pp_instructions pp ic =
         | EF_memcpy _
         | EF_runtime _
         | EF_vload _
-        | EF_vstore _ -> assert false
+        | EF_vstore _
+        | EF_select _ -> assert false
       end
     (* Stackframe, should not occur *)
     | Pallocframe _ -> assert false
